translator/test/incr.ml
@@ -1,0 +1,5 @@
+let new_counter () =
+  let c = ref 0 in
+  let upd i = c := i in
+  let get () = !c in
+  (get, upd)
