theories/libs/Stdlib.v
@@ -4,21 +4,44 @@ From iris.bi Require Import weakestpre.
 From iris.prelude Require Import options.
 Import uPred.
 
-Require Import base lang sugar free eval step wp wp_tactics encode notations.
+From iris Require Import base_logic.lib.gen_heap.
+
+Require Import base lang sugar locations free eval step wp wp_tactics encode notations.
 
 Section StdLib.
   Context `{!osirisGS_gen hlc Σ}.
 
+  (* About integers. *)
   Definition Stdlib__add : val :=
     VClo EnvNil $
       AnonFun "x" $
       EFun "y" $
       EIntAdd (EVar "x") (EVar "y").
 
+  (* About references. *)
+  Definition Stdlib__ref : val :=
+    VClo EnvNil $
+      AnonFun "e" $
+      ERef (EVar "e").
+
+  Definition Stdlib__load : val :=
+    VClo EnvNil $
+      AnonFun "x" $
+      ELoad (EVar "x").
+
+
+
+  (* Putting everything together. *)
   Definition Stdlib :=
     VStruct $
-      EnvCons "+" Stdlib__add EnvNil.
+      EnvCons "+" Stdlib__add $
+      EnvCons "ref" Stdlib__ref $
+      EnvCons "!" Stdlib__load $
+      EnvNil.
 
+
+
+  (* Specifications : integers. *)
   Lemma Stdlib__add__spec s E:
     ∀ v1 v2 i1 i2,
     v1 = VInt (int.repr i1) →
@@ -31,6 +54,33 @@ Section StdLib.
     by rewrite int.add_repr_repr.
   Qed.
 
+
+  (* Specifications : store. *)
+  Lemma Stdlib__ref__spec v (s: stuckness) (E: coPset) :
+    ⊢ WP call Stdlib__ref v @ s; E
+           {{ λ vl, ∃ (ℓ: loc), ℓ ↦ v ∗ ⌜vl = VLoc ℓ ⌝ }}.
+  Proof.
+    wp_call. wp_ref l "[Hl _]".
+    iExists l.
+    iFrame.
+    iPureIntro. reflexivity.
+  Qed.
+
+  Lemma Stdlib__load__spec vl l v s E :
+    {{{ ⌜vl = VLoc l⌝ ∗ l ↦ v }}}
+      call Stdlib__load vl @ s; E
+    {{{ r, RET r; ⌜r = v⌝ ∗ l ↦ v }}}.
+  Proof.
+    iIntros (φ) "[->Hpre] Hφ".
+    wp_call.
+    wp_load "Hpre".
+    wp_use "Hφ".
+    iFrame.
+    iPureIntro. reflexivity.
+  Qed.
+
   Opaque Stdlib__add.
+  Opaque Stdlib__ref.
+  Opaque Stdlib__load.
 End StdLib.
 
